$$
q_i= a_kI_i+ b_k, \forall i \in w_k
$$

$$
\begin{align}
E(a_k, b_k) &= \sum_{i \in w_k}((a_kI_i + b_k-p_i)^2)
\\
&=\sum_{i \in w_k}(a_k^2I_i^2 + b_k^2+p_i^2+2a_kI_ib_k-+2a_kI_ip_i-2b_kp_i)
\end{align}
$$

$$
\begin{align}
\frac{\partial E}{\partial a_k} &= \sum_{i=1}^n(2I_i^2a_k + 2b_kI_i-2I_ip_i) &= 0
\\
\frac{\partial E}{\partial b_k} &= \sum_{i=1}^n(2b_k + 2a_kI_i-2p_i) &= 0
\end{align}
$$

$$
\begin{align}
\sum_{i=1}^nI_i^2a_k + \sum_{i=1}^nI_ib_k &= \sum_{i=1}^nI_ip_i
\\
\sum_{i=1}^n I_ia_k + \sum_{i=1}^n b_k  &= \sum_{i=1}^n p_i
\end{align}
$$

$$
\begin{align}
\sum_{i=1}^n b_k  &= \sum_{i=1}^n p_i - \sum_{i=1}^n I_ia_k
\\
\\
nb_k &= n \overline{p}_i - na_k\mu_k
\\
\\
b_k &=  \overline{p}_i - a_k\mu_k
\end{align}
$$


$$
\begin{pmatrix}
  \sum_{i=1}^nI_i^2a_k & \sum_{i=1}^nI_ib_k \\
  \sum_{i=1}^n I_ia_k & \sum_{i=1}^n b_k \\
\end{pmatrix}
\begin{pmatrix}
  a_k \\
  b_k \\
\end{pmatrix}
=
\begin{pmatrix}
\sum_{i=1}^nI_ip_i \\
\sum_{i=1}^n p_i \\
\end{pmatrix}
$$

$$
\begin{align}
a_k &= \frac
{\begin{vmatrix}
  \sum_{i=1}^nI_ip_i & \sum_{i=1}^nI_i \\
  \sum_{i=1}^n p_i & \sum_{i=1}^n 1 \\
\end{vmatrix}}
{\begin{vmatrix}
  \sum_{i=1}^nI_i^2 & \sum_{i=1}^nI_i \\
  \sum_{i=1}^n I_i & \sum_{i=1}^n 1 \\
\end{vmatrix}}
\\
\\
&=\frac
{\sum_{i=1}^nI_ip_i \sum_{i=1}^n 1 
- 
\sum_{i=1}^nI_i \sum_{i=1}^n p_i}
{\sum_{i=1}^nI_i^2 \sum_{i=1}^n 1
-
\sum_{i=1}^n I_i \sum_{i=1}^n I_i}
\\
\\
&=\frac
{n \sum_{i=1}^nI_ip_i  -  n^2 \mu_k \overline{p}_k}
{n \sum_{i=1}^nI_i^2 - n^2 \mu_k^2}
\\
\\
&= \frac
{\frac{1}{n} \sum_{i=1}^nI_ip_i  -  \mu_k \overline{p}_k}
{\frac{1}{n} \sum_{i=1}^nI_i^2 -  \mu_k^2}
\\
\\
&= \frac
{\frac{1}{n} \sum_{i=1}^nI_ip_i  -  \mu_k \overline{p}_k}
{\frac{1}{n} \sum_{i=1}^n(I_i - \mu_k)^2}
\\
\\
&= \frac
{\frac{1}{n} \sum_{i=1}^nI_ip_i  -  \mu_k \overline{p}_k}
{\sigma^2}
\end{align}
$$






























$$
q_i = a_k I_i + b_k, \forall i \in w_k
$$

$$
E(a_k, b_k) = \sum_{i \in w_k}((a_kI_i + b_k -p_i)^2 + \epsilon a_k^2)
$$

$$
E(a_k, b_k) = \sum_{i=1}^n (a_k^2I_i^2 + b_k^2 + p_i^2 + 2I_ia_kb_k - 2I_ip_ia_k-2p_ib_k)
$$

$$
\frac{\partial E}{\partial a_k}=\sum_{i=1}^n(2I_i^2a_k + 2b_kI_i-2I_ip_i)=0
$$

$$
\frac{\partial E}{\partial b_k}=\sum_{i=1}^n(2b_k + 2a_kI_i-2p_i)=0
$$

$$
\sum_{i=1}^n(I_i^2a_k + I_ib_k)=\sum_{i=1}^nI_i^2a_k+\sum_{i=1}^n I_ib_k=\sum_{i=1}^n(I_ip_i)
$$

$$
\sum_{i=1}^n(I_ia_k+b_k)=\sum_{i=1}^nI_ia_k+\sum_{i=1}^nb_k=\sum_{i=1}^n(p_i)
$$

